code/experimental/he/hestarhs/src/Hacl/Support.hs
@@ -4,18 +4,22 @@ module Hacl.Support where
 
 import Universum hiding (exp, last, (<*>))
 
+import Data.List (splitAt)
+import Numeric (log)
 import System.Random (randomIO, randomRIO)
 
+import Hacl.Bignum
+import Hacl.Raw
 import Lib hiding (crt)
+import Utils
 
 
+-- https://stackoverflow.com/questions/6325576/how-many-iterations-of-rabin-miller-should-i-use-for-cryptographic-safe-primes
 genPrime :: Int -> IO Integer
 genPrime bits = do
-    p <- randomRIO (2 ^ (bits - 4),2 ^ bits)
-    --if isPrime p
+    p <- randomRIO (2 ^ (bits - 4),2 ^ bits) `suchThat` odd
     if isPrimeMR 40 p
       then pure p else genPrime bits
-
 
 legendreSymbol :: Integer -> Integer -> Integer
 legendreSymbol p a = let res = exp p a ((p-1) `div` 2) in if res == p-1 then (-1) else res
@@ -58,3 +62,169 @@ genDataPaillier bits = do
     m1 <- randomRIO (0,n-1)
     m2 <- randomRIO (0,n-1)
     return (p,q,r,m1,m2)
+
+
+log2 :: Integer -> Integer
+log2 x = ceiling $ log (fromIntegral (x+1)) / log 2
+
+fromFacts :: [(Integer,Integer)] -> Integer
+fromFacts = product . map (\(p,i) -> p ^ i)
+
+recombineFacts :: [(Integer,Integer)] -> [(Integer,Integer)]
+recombineFacts xs =
+    let ps = ordNub $ map fst xs in
+    map (\p -> (p,sum $ map snd $ filter ((== p). fst) xs)) ps
+
+flattenFacts :: [(Integer,Integer)] -> [Integer]
+flattenFacts = concatMap (\(p,j) -> replicate (fromIntegral j) p)
+
+factToOrders :: [(Integer,Integer)] -> [Integer]
+factToOrders facts  =
+    sort $ ordNub $ map product $ allCombinations $ flattenFacts facts
+
+orderFact :: [Integer] -> Integer -> Integer -> Integer
+orderFact possibleOrders n g =
+    fromMaybe (error "can't be") $ find (\o -> exp n g o == 1) $ sort possibleOrders
+
+fastFindOrder :: Integer -> Integer -> [Integer] -> IO Integer
+fastFindOrder n g flatFactors = do
+
+    let checkProduct :: [Integer] -> IO Bool
+        checkProduct listPrimes = pure $ exp n g (product listPrimes) == 1
+
+    let loop extraPrms = do
+            if extraPrms == [] then pure []
+            else do
+                resIndex <-
+                    findM (\i -> checkProduct (listRem extraPrms i))
+                          [0..length extraPrms-1]
+                case resIndex of
+                    Nothing -> pure extraPrms
+                    Just i  -> loop (listRem extraPrms i)
+
+    product <$> loop flatFactors
+  where
+    listRem ls i = let (ls1,ls2) = splitAt i ls in ls1 ++ drop 1 ls2
+
+findWithOrder :: Integer -> Integer -> Integer -> [Integer] -> Integer -> IO Integer
+findWithOrder p q n (sort -> posOrders) reqO = do
+    let bn = fromIntegral $ log2 n
+
+    bnZero <- toBignum bn 0
+    bnOne <- toBignum bn 1
+    p' <- toBignum bn p
+    q' <- toBignum bn q
+    n' <- toBignum bn n
+    reqO' <- toBignum bn reqO
+    posOrders' <- mapM (toBignum bn) posOrders
+
+    -- openssl version must be faster
+    let randomBignum = toBignum bn =<< randomRIO (0,n-1)
+
+    e <- toBignum bn 0
+    let orderFactBN :: Bignum -> Bignum -> IO Bignum
+        orderFactBN modulo g =
+            fromMaybe (error "can't be") <$>
+            findM (\o -> do
+                        bnModExp bn bn modulo g o e
+                        bnIsEqual bn bn e bnOne)
+            posOrders'
+
+
+    rem1 <- toBignum bn 0
+    oDivReqo <- toBignum bn 0
+    oModReqo <- toBignum bn 0 -- not used
+    cand <- toBignum bn 0
+    candModP <- toBignum bn 0
+    candModQ <- toBignum bn 0
+    let go i = do
+            g <- randomBignum
+            o <- orderFactBN n' g
+            bnRemainder bn bn o reqO' rem1
+            cond1 <- bnIsEqual bn bn rem1 bnZero
+            if cond1 then do
+                bnDivide bn o reqO' oDivReqo oModReqo
+                bnModExp bn bn n' g oDivReqo cand -- cand = g^(
+                bnRemainder bn bn cand p' candModP
+                bnRemainder bn bn cand q' candModQ
+                o1 <- orderFactBN p' candModP
+                o2 <- orderFactBN q' candModQ
+
+                b1 <- bnIsEqual bn bn o1 o2
+                b2 <- bnIsEqual bn bn o1 reqO'
+                if b1 && b2 then pure cand
+                else go (i+1)
+            else go (i+1)
+
+    fromBignum bn =<< go 0
+
+genDataDGK ::
+       [(Integer, Integer)]
+    -> Int
+    -> IO (Integer, Integer, Integer, Integer, Integer, Integer)
+genDataDGK uFacts bits = do
+    let u = fromFacts uFacts
+    let vbits = 160
+    let ubits = fromIntegral $ log2 u
+    let rbits = bits `div` 2 - ubits - vbits
+    when (rbits < 0) $ error $ "genDataDGK: incorrect params: " <> show (vbits, ubits, rbits)
+
+    v <- genPrime vbits
+    let genR (i::Integer) = do
+          r <- genPrime rbits
+          let p = 2 * u * v * r + 1
+          if isPrimeMR 40 p then pure (r,p) else genR (i+1)
+
+    putTextLn "Generating p"
+    (r_p,p) <- genR 0
+    putTextLn "Generating q"
+    (r_q,q) <- genR 0
+    when (p == q) $ error "p = q"
+    let n = p * q
+
+    let phinFacts =
+            recombineFacts $
+            [(2,2),(r_p,1),(r_q,1),(v,2)] <> uFacts <> uFacts
+    let flatFacts = flattenFacts phinFacts
+
+    a <- randomRIO (0,n-1)
+    unless (exp n a ((p-1)*(q-1)) == 1) $ error "er1"
+    unless (fromFacts phinFacts == (p-1)*(q-1)) $ error "er2"
+
+    let findWithOrd reqO = do
+            g <- randomRIO (0, (p-1)*(q-1))
+            o <- fastFindOrder n g flatFacts
+            if o `mod` reqO == 0 then do
+                let cand = exp n g (o `div` reqO)
+                o1 <- fastFindOrder p (cand `mod` p) flatFacts
+                o2 <- fastFindOrder q (cand `mod` q) flatFacts
+                if o1 == o2 && o1 == reqO then pure cand
+                else findWithOrd reqO
+            else findWithOrd reqO
+
+    putTextLn "Generating g"
+    g <- findWithOrd (u * v)
+    putTextLn "Generating h"
+    h <- findWithOrd v
+
+    pure (p,q,u,v,g,h)
+
+genConsecutivePrms :: Int -> Integer -> [Integer]
+genConsecutivePrms n bound =
+    reverse $ go 0 [] (if even bound then bound+1 else bound+2)
+  where
+    go l xs toTest = if l >= n then xs else
+        if isPrimeMR 40 toTest
+        then go (l+1) (toTest:xs) (toTest+2)
+        else go l xs (toTest+2)
+
+genDataDGKWithPrimes ::
+       Int
+    -> Integer
+    -> Int
+    -> IO ([Integer], Integer, Integer, Integer, Integer, Integer, Integer)
+genDataDGKWithPrimes primeN primeBound bits = do
+    let prms = genConsecutivePrms primeN primeBound
+    let ulog = sum $ map log2 prms
+    (p,q,u,v,g,h) <- genDataDGK (map (,1) prms) bits
+    pure (prms,p,q,u,v,g,h)
