code/experimental/rsapss/include/Hacl_Impl_Bignum_Openssl.c
@@ -3,6 +3,75 @@
 #include <openssl/bn.h>
 
 
+void Hacl_Impl_Bignum_Openssl_ossl_divide(
+  uint32_t aLen,
+  uint64_t *a,
+  uint64_t *b,
+  uint64_t *q,
+  uint64_t *r) {
+    BN_CTX *ctx = BN_CTX_new();
+
+    int aLenBytes = ((int)aLen)*8;
+
+    BIGNUM *bn_a = BN_lebin2bn((unsigned char*) a,aLenBytes,NULL);
+    BIGNUM *bn_b = BN_lebin2bn((unsigned char*) b,aLenBytes,NULL);
+    BIGNUM *bn_q = BN_new();
+    BIGNUM *bn_r = BN_new();
+
+    BN_div(bn_q,bn_r,bn_a,bn_b,ctx);
+
+    if (BN_num_bytes(bn_q) > aLenBytes) {
+        printf ("div 1: nlen: %u, retlen: %u\n", aLen, BN_num_bytes(bn_q));
+        exit(1);
+    }
+
+    if (BN_num_bytes(bn_r) > aLenBytes) {
+        printf ("div 2: nlen: %u, retlen: %u\n", aLen, BN_num_bytes(bn_r));
+        exit(1);
+    }
+
+    BN_bn2lebinpad(bn_q,(unsigned char*)q,aLenBytes);
+    BN_bn2lebinpad(bn_r,(unsigned char*)r,aLenBytes);
+
+    BN_free(bn_a);
+    BN_free(bn_b);
+    BN_free(bn_q);
+    BN_free(bn_r);
+
+    BN_CTX_free(ctx);
+}
+
+void Hacl_Impl_Bignum_Openssl_ossl_mod(
+  uint32_t aLen,
+  uint32_t modLen,
+  uint64_t *a,
+  uint64_t *mod,
+  uint64_t *r) {
+    BN_CTX *ctx = BN_CTX_new();
+
+    int aLenBytes = ((int)aLen)*8;
+    int modLenBytes = ((int)modLen)*8;
+
+    BIGNUM *bn_a = BN_lebin2bn((unsigned char*) a,aLenBytes,NULL);
+    BIGNUM *bn_mod = BN_lebin2bn((unsigned char*) mod,modLenBytes,NULL);
+    BIGNUM *bn_r = BN_new();
+
+    BN_mod(bn_r,bn_a,bn_mod,ctx);
+
+    if (BN_num_bytes(bn_r) > aLenBytes) {
+        printf ("mod: nlen: %u, retlen: %u\n", aLen, BN_num_bytes(bn_r));
+        exit(1);
+    }
+
+    BN_bn2lebinpad(bn_r,(unsigned char*)r,modLenBytes);
+
+    BN_free(bn_a);
+    BN_free(bn_mod);
+    BN_free(bn_r);
+
+    BN_CTX_free(ctx);
+}
+
 void Hacl_Impl_Bignum_Openssl_ossl_mod_add(
   uint32_t nLen,
   uint64_t *n,
