code/experimental/rsapss/Hacl.Impl.Bignum.Openssl.fst
@@ -13,6 +13,38 @@ open Lib.IntTypes
 open Lib.Math.Algebra
 open Lib.Buffer
 
+noextract inline_for_extraction
+val enable_ossl : bool
+let enable_ossl = true
+
+val ossl_divide:
+     #aLen:bn_len
+  -> a:lbignum aLen
+  -> b:lbignum aLen
+  -> q:lbignum aLen
+  -> r:lbignum aLen
+  -> Stack unit
+    (requires fun h ->
+     live h a /\ live h b /\ live h q /\ live h r /\
+     all_disjoint [loc a; loc b; loc q; loc r] /\
+     as_snat h b <> 0)
+    (ensures fun h0 _ h1 -> modifies2 q r h0 h1 /\
+      as_snat h1 q = as_snat h0 a / as_snat h0 b /\
+      as_snat h1 r = as_snat h0 a % as_snat h0 b)
+
+val ossl_mod:
+     #aLen:bn_len{ v aLen * 64 <= max_size_t }
+  -> #modLen:bn_len{ v modLen * 64 <= max_size_t }
+  -> a:lbignum aLen
+  -> mod:lbignum modLen
+  -> res:lbignum modLen
+  -> Stack unit
+    (requires fun h ->
+       live h a /\ live h mod /\ live h res /\
+       disjoint res a /\ disjoint res mod /\ as_snat h mod > 1)
+    (ensures fun h0 _ h1 ->
+       live h1 a /\ live h1 mod /\ live h1 res /\ modifies1 res h0 h1 /\
+       as_snat h1 res = as_snat h0 a % as_snat h0 mod)
 
 val ossl_mod_add:
      #len:bn_len{ (v len + 1) * 64 <= max_size_t}
